WIP: simg alt exp

ems/SimGlobalAlts.v
@@ -22,7 +22,7 @@ Section COMMON.
 
   Variant obs_step (args: string * Any.t * (Any.t -> Prop) * Any.t) (r: ITR -> Prop): ITR -> Prop :=
     | obs_step_syscall
-        fn varg rvs ktr v
+        fn varg rvs v ktr
         (REL: r (ktr v))
         (ARGS: args = (fn, varg, rvs, v))
       :
@@ -75,7 +75,8 @@ Section SRCSTEPS.
   Definition src_step (r: (option (string * Any.t * (Any.t -> Prop) * Any.t)) -> ITR -> Prop):
     ITR -> Prop :=
     fun itr =>
-      (<<TAU: st_step (r None) itr>>) \/ (<<OBS: exists args, obs_step args (r (Some args)) itr>>)
+      (<<TAU: st_step (r None) itr>>) \/
+        (<<OBS: exists arg, forall v, obs_step (arg, v) (r (Some (arg, v))) itr>>)
   .
 
   Definition src_plus (r: (option (string * Any.t * (Any.t -> Prop) * Any.t)) -> ITR -> Prop):
@@ -126,7 +127,7 @@ Section SRCSTEPS.
   Proof.
     i. inv H.
     - econs 1. eapply st_step_mon. 2: eauto. eauto.
-    - des. econs 2. exists args. eapply obs_step_mon. 2: eauto. eauto.
+    - des. econs 2. exists arg. i. eapply obs_step_mon. 2: eauto. eauto.
   Qed.
 
   Lemma src_plus_mon
@@ -137,102 +138,6 @@ Section SRCSTEPS.
   Proof.
     i. eapply st_star_mon. 2: eauto. i; ss. eapply src_step_mon. 2: eauto. eauto.
   Qed.
-
-
-  (* Lemma st_step_comp *)
-  (*       (r0: ITR -> Prop) itr *)
-  (*       (STEP0: st_step r0 itr) *)
-  (*       ktr (CONT0: r0 ktr) *)
-  (*       (r1: ITR -> Prop) *)
-  (*       (STEP1: st_step r1 ktr) *)
-  (*       ctr (CONT1: r1 ctr) *)
-  (*   : *)
-  (*   exists r2, (st_step r2 itr) /\ (r2 ctr). *)
-  (* Proof. *)
-  (*   inv STEP0. *)
-  (*   - inv STEP1. *)
-  (*     + exists  econs 1. *)
-
-  Lemma st_star_st_step_comp
-        (r0: ITR -> Prop) itr
-        (STAR: st_star r0 itr)
-        ktr (CONT0: r0 ktr)
-        (r1: ITR -> Prop)
-        (STEP: st_step r1 ktr)
-        ctr (CONT1: r1 ctr)
-    :
-    exists r2, (st_star r2 itr) /\ (r2 ctr).
-  Proof.
-    revert_until STAR. induction STAR using st_star_ind2. i.
-    { 
-    inv STEP0.
-    - inv STEP1.
-      + exists  econs 1.
-
-
-  Lemma st_star_st_step_comp
-        (r0: ITR -> Prop) itr
-        (STEP0: st_star r0 itr)
-        (r1: ITR -> Prop) ktr
-        (CONT: r0 ktr)
-        (STEP1: st_step r1 ktr)
-    :
-    st_star (fun ktr => (st_step r1 ktr)) itr.
-  Proof.
-    inv STEP0.
-    - inv STEP1.
-      + econs 1.
-
-    econs 1.
-    unfold st_plus, src_plus in *. 
-
-  Lemma st_plus_trans
-        (r0 r1: ITR -> Prop) itr
-        (PLUS: st_plus r0 itr)
-        ktr
-        (CONT: r0 ktr)
-        (STEP: st_plus r1 ktr)
-    :
-    st_plus r1 itr.
-  Proof.
-    unfold st_plus, src_plus in *. 
-
-
-
-    Variant st_step (r: ITR -> Prop): ITR -> Prop :=
-    | st_step_tau
-        ktr
-        (REL: r ktr)
-      :
-      st_step r (tau;; ktr)
-    | st_step_choose
-        X ktr
-        (REL: exists x, r (ktr x))
-      :
-      st_step r (trigger (Choose X) >>= ktr)
-    | st_step_take
-        X ktr
-        (REL: forall x, r (ktr x))
-      :
-      st_step r (trigger (Take X) >>= ktr)
-  .
-
-  Inductive st_star (r: ITR -> Prop): ITR -> Prop :=
-  | st_star_base itr (REL: r itr): st_star r itr
-  | st_star_step itr (REL: st_step (fun ktr => st_star r ktr) itr): st_star r itr
-  .
-
-  Definition src_step (r: (option (string * Any.t * (Any.t -> Prop) * Any.t)) -> ITR -> Prop):
-    ITR -> Prop :=
-    fun itr =>
-      (<<TAU: st_step (r None) itr>>) \/ (<<OBS: exists args, obs_step args (r (Some args)) itr>>)
-  .
-
-  Definition src_plus (r: (option (string * Any.t * (Any.t -> Prop) * Any.t)) -> ITR -> Prop):
-    ITR -> Prop := (st_star (fun ktr => src_step r ktr))
-  .
-
-  Definition st_plus (r: ITR -> Prop): ITR -> Prop := src_plus (fun args ktr => (args = None) /\ (r ktr)).
 
 End SRCSTEPS.
 
@@ -260,11 +165,23 @@ Section TGTSTEPS.
       tt_step r (trigger (Take X) >>= ktr)
   .
 
+  Inductive tt_star (r: ITR -> Prop): ITR -> Prop :=
+  | tt_star_base itr (REL: r itr): tt_star r itr
+  | tt_star_step itr (REL: tt_step (fun ktr => tt_star r ktr) itr): tt_star r itr
+  .
+
   Definition tgt_step (r: (option (string * Any.t * (Any.t -> Prop) * Any.t)) -> ITR -> Prop):
     ITR -> Prop :=
     fun itr =>
-      (<<TAU: tt_step (r None) itr>>) \/ (<<OBS: exists args, obs_step args (r (Some args)) itr>>)
+      (<<TAU: tt_step (r None) itr>>) \/
+        (<<OBS: exists arg, forall v, obs_step (arg, v) (r (Some (arg, v))) itr>>)
   .
+
+  Definition tgt_plus (r: (option (string * Any.t * (Any.t -> Prop) * Any.t)) -> ITR -> Prop):
+    ITR -> Prop := (tt_star (fun ktr => tgt_step r ktr))
+  .
+
+  Definition tt_plus (r: ITR -> Prop): ITR -> Prop := tgt_plus (fun args ktr => (args = None) /\ (r ktr)).
 
   (* properties *)
   Lemma tt_step_mon
@@ -276,6 +193,30 @@ Section TGTSTEPS.
     i. inv H; econs; eauto. des. eauto.
   Qed.
 
+  Lemma tt_star_ind2 (r: ITR -> Prop) (P: ITR -> Prop)
+        (BASE: forall itr (REL: r itr), P itr)
+        (STEP: forall itr (REL: tt_step (fun ktr => (<<STAR: tt_star r ktr>>) /\ (<<IH: P ktr>>)) itr),
+            P itr)
+    :
+    forall itr (STAR: tt_star r itr), P itr.
+  Proof.
+    fix IH 2. i. inv STAR. eauto.
+    eapply STEP. inv REL.
+    { econs 1. split; auto. }
+    { econs 2. i. split; auto. }
+    { econs 3. des. exists x. split; auto. }
+  Qed.
+
+  Lemma tt_star_mon
+        (r0 r1: ITR -> Prop) itr
+        (MON: forall itr, (r0 itr) -> (r1 itr))
+    :
+    (tt_star r0 itr) -> (tt_star r1 itr).
+  Proof.
+    i. induction H using tt_star_ind2. econs 1; eauto.
+    econs 2. eapply tt_step_mon. 2: eauto. i; ss. des. auto.
+  Qed.
+
   Lemma tgt_step_mon
         (r0 r1: (option (string * Any.t * (Any.t -> Prop) * Any.t)) -> ITR -> Prop) itr
         (MON: forall args itr, (r0 args itr) -> (r1 args itr))
@@ -284,7 +225,16 @@ Section TGTSTEPS.
   Proof.
     i. inv H.
     - econs 1. eapply tt_step_mon. 2: eauto. eauto.
-    - des. econs 2. exists args. eapply obs_step_mon. 2: eauto. eauto.
+    - des. econs 2. exists arg. i. eapply obs_step_mon. 2: eauto. eauto.
+  Qed.
+
+  Lemma tgt_plus_mon
+        (r0 r1: (option (string * Any.t * (Any.t -> Prop) * Any.t)) -> ITR -> Prop) itr
+        (MON: forall args itr, (r0 args itr) -> (r1 args itr))
+    :
+    (tgt_plus r0 itr) -> (tgt_plus r1 itr).
+  Proof.
+    i. eapply tt_star_mon. 2: eauto. i; ss. eapply tgt_step_mon. 2: eauto. eauto.
   Qed.
 
 End TGTSTEPS.
@@ -297,15 +247,17 @@ Section EXP_SIM.
 
   Definition _simg_alt_exp
              (simg_alt_exp: forall R0 R1 (RR: R0 -> R1 -> Prop), wfo.(T) -> (itree eventE R0) -> (itree eventE R1) -> Prop)
-             {R0 R1} (RR: R0 -> R1 -> Prop) (f_tgt: wfo.(T)): (itree eventE R0) -> (itree eventE R1) -> Prop :=
+             {R0 R1} (RR: R0 -> R1 -> Prop) (exp: wfo.(T)): (itree eventE R0) -> (itree eventE R1) -> Prop :=
     fun itr_src itr_tgt =>
-      (<<RET: exists rt, (<<RETTGT: is_ret rt itr_tgt>>) ->
-                    (<<RETSRC: st_star (fun ktr => exists rs, (is_ret rs ktr) /\ (RR rs rt)) itr_src>>)>>)
-      /\
-        (
-          (<<STAR: (tt_step (fun ktr_tgt => (st_star (fun ktr_src => exists f_tgt0, (simg_alt_exp _ _ RR f_tgt0 ktr_src ktr_tgt) /\ (wfo.(lt) f_tgt0 f_tgt)) itr_src)) itr_tgt)>>)
-          \/
-            (<<PLUS: (tgt_step (fun targs ktr_tgt => (src_plus (fun sargs ktr_src => exists f_tgt0, (simg_alt_exp _ _ RR f_tgt0 ktr_src ktr_tgt) /\ (targs = sargs)) itr_src)) itr_tgt)>>)
+      (exists rt rs, (<<TGT: is_ret rt itr_tgt>>) /\ (<<SRC: is_ret rs itr_src>>) /\ (<<RET: RR rs rt>>))
+      \/
+        ((<<TGT: (tt_step (fun ktr_tgt => (st_star (fun ktr_src => exists exp0, (simg_alt_exp _ _ RR exp0 ktr_src ktr_tgt) /\ (wfo.(lt) exp0 exp)) itr_src)) itr_tgt)>>)
+         \/
+           (<<SRC: (st_step (fun ktr_src => (tt_star (fun ktr_tgt => exists exp0, (simg_alt_exp _ _ RR exp0 ktr_src ktr_tgt) /\ (wfo.(lt) exp0 exp)) itr_tgt)) itr_src)>>)
+         \/
+           (<<TPLUS: (tgt_plus (fun targ ktr_tgt => (src_plus (fun sarg ktr_src => (<<EQ: targ = sarg>>) -> exists exp0, (simg_alt_exp _ _ RR exp0 ktr_src ktr_tgt)) itr_src)) itr_tgt)>>)
+         \/
+           (<<SPLUS: (src_plus (fun sarg ktr_src => (tgt_plus (fun targ ktr_tgt => (<<EQ: sarg = targ>>) -> exists exp0, (simg_alt_exp _ _ RR exp0 ktr_src ktr_tgt)) itr_tgt)) itr_src)>>)
         )
   .
 
@@ -313,22 +265,63 @@ Section EXP_SIM.
 
   Lemma simg_alt_exp_mon: monotone6 _simg_alt_exp.
   Proof.
-    ii. inv IN. des.
-    { unfold _simg_alt_exp. split; eauto.
-      left. eapply tt_step_mon. 2: eauto. i; ss. eapply st_star_mon. 2: eauto. i; ss.
-      des. eauto.
-    }
-    { unfold _simg_alt_exp. split; eauto.
-      right. eapply tgt_step_mon. 2: eauto. i; ss. eapply src_plus_mon. 2: eauto. i; ss.
-      des. eauto.
-    }
+    ii. inv IN.
+    { left. eauto. }
+    right. des; [left | right; left | do 2 right; left | do 3 right].
+    { eapply tt_step_mon. 2: eauto. i; ss. eapply st_star_mon. 2: eauto. i; ss. des; eauto. }
+    { eapply st_step_mon. 2: eauto. i; ss. eapply tt_star_mon. 2: eauto. i; ss. des; eauto. }
+    { eapply tgt_plus_mon. 2: eauto. i; ss. eapply src_plus_mon. 2: eauto. i; ss.
+      specialize (H0 H1). des; eauto. }
+    { eapply src_plus_mon. 2: eauto. i; ss. eapply tgt_plus_mon. 2: eauto. i; ss.
+      specialize (H0 H1). des; eauto. }
   Qed.
 
   Hint Resolve simg_alt_exp_mon: paco.
   Hint Resolve cpn6_wcompat: paco.
 
-
 End EXP_SIM.
 Hint Unfold simg_alt_exp.
 Hint Resolve simg_alt_exp_mon: paco.
 Hint Resolve cpn6_wcompat: paco.
+
+(* Section EXP_SIM. *)
+
+(*   Variable wfo: WF. *)
+
+(*   Definition _simg_alt_exp *)
+(*              (simg_alt_exp: forall R0 R1 (RR: R0 -> R1 -> Prop), wfo.(T) -> (itree eventE R0) -> (itree eventE R1) -> Prop) *)
+(*              {R0 R1} (RR: R0 -> R1 -> Prop) (f_tgt: wfo.(T)): (itree eventE R0) -> (itree eventE R1) -> Prop := *)
+(*     fun itr_src itr_tgt => *)
+(*       (<<RET: exists rt, (<<RETTGT: is_ret rt itr_tgt>>) -> *)
+(*                     (<<RETSRC: st_star (fun ktr => exists rs, (is_ret rs ktr) /\ (RR rs rt)) itr_src>>)>>) *)
+(*       /\ *)
+(*         ( *)
+(*           (<<STAR: (tt_step (fun ktr_tgt => (st_star (fun ktr_src => exists f_tgt0, (simg_alt_exp _ _ RR f_tgt0 ktr_src ktr_tgt) /\ (wfo.(lt) f_tgt0 f_tgt)) itr_src)) itr_tgt)>>) *)
+(*           \/ *)
+(*             (<<PLUS: (tgt_step (fun targs ktr_tgt => (src_plus (fun sargs ktr_src => exists f_tgt0, (simg_alt_exp _ _ RR f_tgt0 ktr_src ktr_tgt) /\ (targs = sargs)) itr_src)) itr_tgt)>>) *)
+(*         ) *)
+(*   . *)
+
+(*   Definition simg_alt_exp: forall R0 R1 (RR: R0 -> R1 -> Prop), wfo.(T) -> (itree eventE R0) -> (itree eventE R1) -> Prop := paco6 _simg_alt_exp bot6. *)
+
+(*   Lemma simg_alt_exp_mon: monotone6 _simg_alt_exp. *)
+(*   Proof. *)
+(*     ii. inv IN. des. *)
+(*     { unfold _simg_alt_exp. split; eauto. *)
+(*       left. eapply tt_step_mon. 2: eauto. i; ss. eapply st_star_mon. 2: eauto. i; ss. *)
+(*       des. eauto. *)
+(*     } *)
+(*     { unfold _simg_alt_exp. split; eauto. *)
+(*       right. eapply tgt_step_mon. 2: eauto. i; ss. eapply src_plus_mon. 2: eauto. i; ss. *)
+(*       des. eauto. *)
+(*     } *)
+(*   Qed. *)
+
+(*   Hint Resolve simg_alt_exp_mon: paco. *)
+(*   Hint Resolve cpn6_wcompat: paco. *)
+
+
+(* End EXP_SIM. *)
+(* Hint Unfold simg_alt_exp. *)
+(* Hint Resolve simg_alt_exp_mon: paco. *)
+(* Hint Resolve cpn6_wcompat: paco. *)
