ems/SimGlobalExplicit2AltExp.v
@@ -26,9 +26,24 @@ Section PROOF.
           (e_src e_tgt: wf_exp.(T))
           (SIM: simg_exp wf_exp RR e_src e_tgt (itr_src) (itr_tgt))
     :
-    exists wfo f_tgt,
-      simg_alt_exp wfo RR f_tgt itr_src itr_tgt.
+    exists wfo exp,
+      simg_alt_exp wfo RR exp itr_src itr_tgt.
   Proof.
+    set (wfo := prod_WF wf_exp wf_exp). Local Opaque prod_WF.
+    move wfo before RR. exists wfo. exists (e_tgt, e_src).
+    ginit. revert_until wfo. gcofix CIH. i.
+    move e_tgt before CIH. revert_until e_tgt. pattern e_tgt. revert e_tgt.
+    apply (well_founded_induction wf_exp.(wf)). intros e_tgt IHt. i.
+    punfold SIM. inv SIM.
+    { gstep. left. esplits; eauto. all: econs; eauto. }
+    { gstep. right. do 3 right. econs 1. right. exists (fn, varg, rvs). i. econs; eauto.
+      econs 1. right. exists (fn, varg, rvs). i. econs; eauto.
+      i. inversion H. specialize (SIM0 v v0 H1). destruct SIM0; clarify.
+      exists (f_tgt0, f_src0). gfinal. left. eapply CIH; eauto.
+    }
+    { destruct SIM0 as [SIM | SIM]; clarify. 
+
+    
 
 
 End PROOF.
